imp_system/mem/MemI.v
@@ -4,54 +4,30 @@ Set Implicit Arguments.
 Set Typeclasses Depth 5.
 
 Module Mem.
-
-  (* Definition t : Type := mblock -> option (Z -> val). *)
   Record t : Type := mk {
-    cnts : mblock -> Z -> option val;
+    cnts : mblock → Z → option val;
     nb : mblock;
-    (*** Q : wf conditions like nextmblock_noaccess ? ***)
-    (*** A : Unlike in CompCert, the memory object will not float in various places in the program.
-            It suffices to state wf only inside Mem module. (probably by utilizing URA.wf)
-     ***)
   }
   .
 
-  Definition wf (m0 : t) : Prop := forall blk ofs (LT : (blk < m0.(nb))%nat), m0.(cnts) blk ofs = None.
+  Definition wf (m0 : t) : Prop := ∀ blk ofs (LT : (blk < m0.(nb))%nat), m0.(cnts) blk ofs = None.
 
-  Definition alloc (m0 : Mem.t) (sz : Z) : (mblock * Mem.t) :=
-    ((m0.(nb)),
+  Definition alloc (m0 : Mem.t) (sz : Z) : mblock * Mem.t :=
+    ((nb m0),
      Mem.mk (update (m0.(cnts)) (m0.(nb))
                     (fun ofs => if (0 <=? ofs)%Z && (ofs <? sz)%Z then Some (Vundef) else None))
             (S m0.(nb))
-    )
-  .
+    ).
 
   Opaque Z.ltb Z.leb Z.mul Z.eq_dec Nat.eq_dec.
-  (* Definition empty : t := mk (update (fun _ _ => None) 0 (fun ofs => if dec ofs 0%Z then Some Vundef else None)) 0. *)
-  Definition empty : t := mk (fun _ _ => None) 0.
-  (* Let empty2 : t := Eval compute in *)
-  (*   let m0 := mk (fun _ _ => None) 0 in *)
-  (*   let (_, m1) := alloc m0 1%Z in *)
-  (*   m1 *)
-  (* . *)
-  (*** shoul allocated with Vundef, not 0 ***)
 
-  (*** TODO : Unlike CompCert, this "free" function does not take offset.
-       In order to support this, we need more sophisticated RA. it would be interesting.
-   ***)
-  (* Definition free (m0 : Mem.t) (b : mblock) : option (Mem.t) := *)
-  (*   match m0.(cnts) b ofs0 with *)
-  (*   | Some _ => Some (Mem.mk (update m0.(cnts) b (fun _ => None)) m0.(nb)) *)
-  (*   | _ => None *)
-  (*   end *)
-  (* . *)
+  Definition empty : t := mk (fun _ _ => None) 0.
 
   Definition free (m0 : Mem.t) := fun '(b,ofs) =>
     match m0.(cnts) b ofs with
     | Some _ => Some (Mem.mk (update m0.(cnts) b (update (m0.(cnts) b) ofs None)) m0.(nb))
     | _ => None
-    end
-  .
+    end.
 
   Definition load (m0 : Mem.t) := fun '(b,ofs) =>
     m0.(cnts) b ofs.
@@ -62,16 +38,12 @@ Module Mem.
                                              then Some v
                                              else m0.(cnts) _b _ofs) m0.(nb))
     | _ => None
-    end
-  .
+    end.
 
   Definition valid_ptr (m0 : Mem.t) := fun '(b,ofs) =>
     is_some (m0.(cnts) b ofs).
 
-(*** NOTE : Probably we can support comparison between nullptr and 0 ***)
-(*** NOTE : Unlike CompCert, we don't support comparison with weak_valid_ptr (for simplicity) ***)
-
-  Definition load_mem (csl : string -> bool) (genv : GEnv.t) : Mem.t :=
+  Definition load_mem (csl : string → bool) (genv : GEnv.t) : Mem.t :=
     Mem.mk
       (fun blk ofs =>
          do '(g, gd) <- (List.nth_error genv blk);
@@ -83,19 +55,10 @@ Module Mem.
            if (dec ofs 0%Z) then Some (Vint gv) else None
           | _ => None
          end)
-      (*** TODO : This simplified model doesn't allow function pointer comparsion.
-           To be more faithful, we need to migrate the notion of "permission" from CompCert.
-           CompCert expresses it with "nonempty" permission.
-       ***)
-      (*** TODO : When doing so, I would like to extend val with "Vfid (id : string)" case.
-           That way, I might be able to support more higher-order features (overriding, newly allocating function)
-       ***)
-      (List.length genv)
-  .
+      (List.length genv).
 
   Definition mem_pad (m0 : Mem.t) (delta : nat) : Mem.t :=
-    Mem.mk m0.(Mem.cnts) (m0.(Mem.nb) + delta)
-  .
+    Mem.mk m0.(Mem.cnts) (m0.(Mem.nb) + delta).
 
   Definition vcmp (m0 : Mem.t) (x y : val) : option bool :=
     match x, y with
@@ -114,17 +77,16 @@ Module Mem.
       else None
     | _, _ => None
     end.
-
 End Mem.
 
 Module MemI. Section MemI.
   Context `{!crisG Γ Σ α β τ _S _I, !concG}.
 
-  Definition scopes := ["Mem"].
-  Definition v_mem := "Mem" ↯ "mem".
+  Definition scopes : gmultiset string := {[+"Mem"+]}.
+  Definition v_mem : key := "Mem" ↯ "mem".
 
   Definition alloc : list val → itree crisE val :=
-    fun arg =>
+    λ arg,
       'sz : Z <- (pargs [Tint] arg)?;;
       mem <- trigger (SGet v_mem);; mem <- mem↓?;;
       if (Z_le_gt_dec 0 sz && Z_lt_ge_dec (8 * sz) modulus_64)
@@ -133,8 +95,7 @@ Module MemI. Section MemI.
             let (blk, mem1) := Mem.alloc mem0 sz in
             trigger (SPut v_mem mem1↑);;;
             Ret (Vptr (blk, 0%Z)))
-      else triggerUB
-. 
+      else triggerUB. 
 
   Definition free : list val → itree crisE val :=
     λ arg,
@@ -145,8 +106,8 @@ Module MemI. Section MemI.
       Ret (Vint 0)
   . 
 
-  Definition load: list val -> itree crisE val :=
-    fun arg =>      
+  Definition load: list val → itree crisE val :=
+    λ arg,      
       bofs <- (pargs [Tptr] arg)?;;        
       mem <- trigger (SGet v_mem);; mem <- mem↓?;;
       v <- (Mem.load mem bofs)?;;
@@ -154,7 +115,7 @@ Module MemI. Section MemI.
   .
 
   Definition store : list val → itree crisE val :=
-    fun arg =>
+    λ arg,
       '(bofs, v): _ <- (pargs [Tptr; Tuntyped] arg)?;;
       mem <- trigger (SGet v_mem);; mem <- mem↓?;;
       mem1 <- (Mem.store mem bofs v)?;;
@@ -163,41 +124,46 @@ Module MemI. Section MemI.
   .
 
   Definition cmp : list val → itree crisE val :=
-    fun arg =>
+    λ arg,
       '(v0, v1): _ <- (pargs [Tuntyped; Tuntyped] arg)?;;
       mem <- trigger (SGet v_mem);; mem <- mem↓?;;
       'b: bool <- (Mem.vcmp mem v0 v1)?;;
       Ret (Vint (if b then 1 else 0))
   .
 
-  Definition cas: list val -> itree crisE val :=
-    fun arg =>
-      ' (bofs, (v_old, v_new)): _ <- (pargs [Tptr; Tuntyped; Tuntyped] arg)?;;
-      'v_cur: val <- ccallU MemHdr.load [Vptr bofs];;
-      'succ: val <- ccallU MemHdr.cmp [v_cur; v_old];;
-      (if (dec succ (Vint 1))
+  Definition cas: list val → itree crisE val :=
+    λ arg,
+      '(bofs, (v_old, v_new)) : _ <- (pargs [Tptr; Tuntyped; Tuntyped] arg)?;;
+      'v_cur : val <- ccallU MemHdr.load [Vptr bofs];;
+      'succ : val <- ccallU MemHdr.cmp [v_cur; v_old];;
+      (if (decide (succ = (Vint 1)))
        then ccallU MemHdr.store [Vptr bofs; v_new]
        else Ret Vundef);;;
-      Ret v_cur
-  .
-  
-  Definition fnsems : alist (option string) (fnsem_type (option fspec * fbody)) :=
-    [(Some MemHdr.alloc, (false, wmask_all, scopes, (None, (cfunU alloc)))) ;
-     (Some MemHdr.free,  (false, wmask_all, scopes, (None, (cfunU free)))) ;
-     (Some MemHdr.load,  (false, wmask_all, scopes, (None, (cfunU load)))) ;
-     (Some MemHdr.store, (false, wmask_all, scopes, (None, (cfunU store)))) ;
-     (Some MemHdr.cmp,   (false, wmask_all, scopes, (None, (cfunU cmp)))) ;
-     (Some MemHdr.cas,   (false, wmask_all, scopes, (None, (cfunU cas))))].
+      Ret v_cur.
 
-  Program Definition smod csl genv : SMod.t :=
-    {|
-      SMod.scopes := scopes;
-      SMod.fnsems := fnsems ;
-      SMod.initial_st := [(v_mem, (Mem.load_mem csl genv)↑)];
-    |}
-  .
-  Solve All Obligations with prove_scope.
-  Next Obligation. prove_nodup. Qed.
+  Definition fnsems : gmap (option string) (option (emask * (option fspec * fbody))) :=
+    {[Some MemHdr.alloc := Some (msk_real (msk_scp scopes msk_true), (None, (cfunU alloc)));
+      Some MemHdr.free := Some (msk_real (msk_scp scopes msk_true), (None, (cfunU free)));
+      Some MemHdr.load := Some (msk_real (msk_scp scopes msk_true), (None, (cfunU load)));
+      Some MemHdr.store := Some (msk_real (msk_scp scopes msk_true), (None, (cfunU store)));
+      Some MemHdr.cmp := Some (msk_real (msk_scp scopes msk_true), (None, (cfunU cmp)));
+      Some MemHdr.cas := Some (msk_real (msk_scp scopes msk_true), (None, (cfunU cas)))]}.
 
-  Definition t csl genv := Seal.sealing CRIS (SMod.to_mod sp_none (smod csl genv)).
+  Program Definition smod csl genv : SMod.t := {|
+    SMod.scopes := scopes;
+    SMod.fnsems := fnsems;
+    SMod.initial_st := {[v_mem := Some (Mem.load_mem csl genv)↑]};
+  |}.
+  Solve Obligations with auto.
+  Next Obligation.
+    i.
+    rewrite ?omap_insert /= omap_empty.
+    mod_tac scope_solver.
+  Qed.
+  Next Obligation.
+    i. mod_tac scope_solver.
+  Qed.
+
+  (* TODO : Sealing *)
+  Definition t csl genv := (SMod.to_mod ∅ (smod csl genv)).
 End MemI. End MemI.
