theories/common/Events.v
@@ -300,9 +300,28 @@ Proof using.
     repeat f_equal. extensionality x. rewrite bind_ret_l. eauto.
 Qed.
 
+(* Masks for sandboxing *)
 Definition emask {Σ : GRA} : Type := ∀ X, crisE X → bool.
 
-Definition img_msk `{Σ: GRA} (msk: emask): Prop :=
+Definition msk_true `{Σ : GRA} : emask := λ X e, true.
+
+Definition msk_scp `{Σ : GRA} (scp : gmultiset string) (msk : emask) : emask :=
+  λ X e,
+    match e with
+    | inr1 (inr1 (inl1 (SPut k v))) => decide (k.1 ∈ scp)
+    | inr1 (inr1 (inl1 (SGet k))) => decide (k.1 ∈ scp)
+    | _ => msk X e
+    end.
+
+Definition msk_real `{Σ : GRA} (msk : emask) : emask :=
+  λ X e,
+    match e with
+    | inl1 (Assume P) => false
+    | inr1 (inr1 (inr1 (Take X))) => excluded_middle_informative (∃ P : Prop, X = P)
+    | _ => msk X e
+    end.
+
+Definition img_msk `{Σ : GRA} (msk : emask) : Prop :=
   (∀ T, msk _ (subevent _ (Take T)) = true)
   ∧ (∀ T, msk _ (subevent _ (Choose T)) = true)
   ∧ (∀ P, msk _ (subevent _ (Assume P)) = true)
