theories/common/CRIS.v
@@ -4,6 +4,7 @@ From iris.proofmode Require Export proofmode.
 Require Export FSpec Sp.
 Require Export SMod Mod.
 Require Export ISim ISimFacts WSim WSimFacts ISimNotations WSimNotations.
+Require Export TacticsCommon.
 Require Export Tactics TacticsInit IrisTactics.
 
 Require Export CallFilter CtxRefine CtxRefineFacts ClosedAdequacy MainAdequacy.
